add1 type derivation more readable

formal-proofs/LetTick/Evaluation.lean
@@ -1,8 +1,11 @@
+import Resources.Definitions
+import LetTick.Language
+
 --Evaluation judgement
 inductive Evaluation : Prog → ResourceDemand → Prop :=
-  | e_tick_pos (k : Int) (pos : k ≥ 0):
-    Evaluation (.tick k) (⟨k, pos⟩, 0) 
-  | e_tick_neg (k : Int) (neg: k < 0):
-    Evaluation (.tick (abs k)) (⟨(abs k), abs_nonneg k⟩, 0)
+  | e_tick_pos (k : Nat): --tick with positive resources
+    Evaluation (.tick k) (k, 0) 
+  | e_tick_neg (k : Int): --tick with negative resources
+    Evaluation (.tick (abs k)) (0, Int.natAbs k)
   | e_let {e_1 e_2 : Prog} {r_1 r_2 : ResourceDemand} (eval_e_1 : Evaluation e_1 r_1) (eval_e_2 : Evaluation e_2 r_2)
     : Evaluation (.letexp e_1 e_2) (r_1 ▹ r_2)
