formal-proofs/LetTick/Language.lean
@@ -6,5 +6,5 @@ inductive BaseType :=
 def RAType := BaseType × ResourceDemand
 
 inductive Prog :=
-  | tick (k : Int)
-  | letexp (e_1 e_2 : Prog)
+  | tick (k : Int) -- tick k
+  | letexp (e_1 e_2 : Prog) -- let _ = e_1 in e_2
