formal-proofs/LetTick/Soundness.lean
@@ -1,3 +1,15 @@
+import Resources.Definitions
+import LetTick.Language
+import LetTick.Typing
+import LetTick.Evaluation
+
+open ResourceDemand
 --Proof of soundness. Theorem 3.5
 theorem soundness (p : Prog) (r_1 r_2 : ResourceDemand) (t : BaseType) 
-  : Evaluation p r_1 → Typing p t r_2 → r_2 ≽ r_1 := by sorry
+  : Evaluation p r_1 → Typing p t r_2 → r_2 ≽ r_1 := by 
+  intros e_H t_H
+  cases p 
+  cases e_H
+  cases t_H
+  rename_i k rel
+  simp[relaxation_of]; simp[init]; simp[resid]
