formal-proofs/Resources/Monoid.lean
@@ -4,15 +4,13 @@ open ResourceDemand
 
 --(0, 0) is left unit under sequencing
 theorem left_unit (p : ResourceDemand) : ((0, 0) ▹ p) = (p.init, p.resid) := by
-  simp [resid]
-  simp [sequence]
-
+  simp[init]; simp[resid]
 
 
 --(0, 0) is right unit under sequencing
 theorem right_unit (p: ResourceDemand) : (p ▹ (0, 0)) = p := by
-  sorry
+  simp[init]; simp[resid]
 
 --sequencing is associative
 theorem associative (p q r : ResourceDemand) : (p ▹ (q ▹ r)) = ((p ▹ q) ▹ r) := by
-  sorry
+  simp[init]; simp[resid];
